memmgr/verif_malloc_free.v
@@ -18,26 +18,55 @@ forward_if. (*! if nbytes > t'3 !*)
   { (* precond *) destruct H. split; try assumption. } 
   Intros p.
   forward. (*! return t'1 !*) 
-  Exists p. entailer!.
+  Exists p.
+  assert (guaranteed lens n = false) by (apply large_not_guaranteed; auto).
+  destruct (guaranteed lens n).
+  inversion H1.
+  assert (Hlem: bin2sizeZ(BINS - 1) < n -> size2binZ n >= BINS ) by 
+      admit. (* TODO lemma or corollary of claims *)
+  apply Hlem in H0; clear Hlem.
+  assert (size2binZ n <? BINS = false) by
+      (bdestruct (size2binZ n <? BINS); [ rep_omega |  reflexivity]).
+  destruct (eq_dec p nullval); entailer.
+  simple_if_tac.
+  inversion H2.
+  cancel.
 - (* case nbytes <= bin2size(BINS-1) *)
   forward_call(n, gv, lens).  (*! t'2 = malloc_small(nbytes) !*)
   { (* precond *)  destruct H. split; try rep_omega. }
   Intros p.
   forward. (*! result = t'2 !*)
   Exists p. 
+  assert (size2binZ n <? BINS = true) by admit. (* TODO lemma or corollary of claims *)
+  destruct (eq_dec p nullval); entailer.
+  simple_if_tac.
   entailer!.
-Qed.
+  Intros lens'. 
+  bdestruct (size2binZ n <? BINS).
+  Exists lens'.
+  entailer.
+  inversion H1.
+  all: fail.
+Admitted.
 
-Lemma body_free:  semax_body Vprog Gprog f_free free_spec'.
+Lemma body_free:  semax_body Vprog Gprog f_free free_spec_R'.
 Proof. 
 start_function. 
-forward_if (PROP()LOCAL()SEP(mem_mgr gv)). (*! if (p != NULL) !*)
+
+
+
+forward_if (PROP()LOCAL()                          (*! if (p != NULL) !*)
+                SEP (if eq_dec p nullval
+                     then mem_mgr_R gv lens 
+                     else if size2binZ n <? BINS
+                          then mem_mgr_R gv (incr_lens lens (size2binZ n) 1)
+                          else mem_mgr_R gv lens )). 
 - (* typecheck *) if_tac; entailer!.
 - (* case p!=NULL *)
   apply semax_pre with 
    (PROP ( )
      LOCAL (temp _p p; gvars gv)
-     SEP (mem_mgr gv;  malloc_token' Ews n p * memory_block Ews n p)).
+     SEP (mem_mgr_R gv lens;  malloc_token' Ews n p * memory_block Ews n p)).
   { if_tac; entailer!. }
   assert_PROP ( 0 <= n <= Ptrofs.max_unsigned - WORD ) by entailer!. 
   sep_apply (from_malloc_token'_and_block n p); auto.
@@ -53,11 +82,30 @@ forward_if (PROP()LOCAL()SEP(mem_mgr gv)). (*! if (p != NULL) !*)
   forward_call(BINS - 1). (*! t'1 = bin2size(BINS - 1) !*)
   { (* precond *) rep_omega. } 
   deadvars!.
-  forward_if (PROP () LOCAL () SEP (mem_mgr gv)). (*! if s <= t'1 !*)
+  forward_if (PROP()LOCAL()               (*! if s <= t'1 !*)
+              SEP (if size2binZ n <? BINS
+                   then mem_mgr_R gv (incr_lens lens (size2binZ n) 1)
+                   else mem_mgr_R gv lens )). 
   -- (* case s <= bin2sizeZ(BINS-1) *)
-    forward_call(p,s,n,gv). (*! free_small(p,s) !*) 
+    forward_call(p,s,n,gv,lens). (*! free_small(p,s) !*) 
     { (* preconds *) split3; try omega; try assumption. }
-    entailer!. if_tac. entailer. omega.
+    destruct (zle s (bin2sizeZ (BINS - 1))). 
+    ++ bdestruct(size2binZ n <? BINS); try rep_omega.
+       +++ (* small chunk *) entailer!.
+       +++ (* contradict *)
+
+         apply H4 in l.
+         subst.
+         apply Znot_lt_ge in H8.
+         assert (H8contra: size2binZ n < BINS). {
+           clear H4 H H6 H8.
+           assert(n <= bin2sizeZ (BINS - 1)) by rep_omega.
+           apply bin2size2bin_small_equiv; rep_omega.
+         }
+         rep_omega.
+
+    ++ rep_omega.
+
   -- (* case s > bin2sizeZ(BINS-1) *)
     if_tac; try omega.
     (*! munmap( p-(WASTE+WORD), s+WASTE+WORD ) !*)
@@ -70,10 +118,25 @@ forward_if (PROP()LOCAL()SEP(mem_mgr gv)). (*! if (p != NULL) !*)
       entailer!.
     + rep_omega.
     + entailer!.
+
+      ++ bdestruct(size2binZ n <? BINS); try rep_omega.
+         +++ admit. (* contra *)
+
+         +++ entailer.
+
+(* TODO seems disorganized *)
+-- 
+
+destruct (eq_dec p nullval); try contradiction.
+entailer.
+
+
 - (* case p == NULL *) 
   forward. (*! skip !*)
-  entailer!.
-Qed.
+  entailer.
+
+all: fail.
+Admitted.
 
 
 Definition module : list semax_body_proof := 
